splitting/splitting_tactics.v
@@ -14,6 +14,147 @@ Implicit Types Γ : env PROP.
 Implicit Types Δ : envs PROP.
 Implicit Types P Q : PROP.
 
+Lemma tac_eval Δ Q Q' :
+  (∀ (Q'':=Q'), Q'' ⊢ Q) → (* We introduce [Q''] as a let binding so that
+    tactics like `reflexivity` as called by [rewrite //] do not eagerly unify
+    it with [Q]. See [test_iEval] in [tests/proofmode]. *)
+  envs_entails Δ Q' → envs_entails Δ Q.
+Proof. intro H. by rewrite envs_entails_eq -H. Qed.
+
+Lemma tac_eval_in Δ i p c P P' Q :
+  envs_lookup_with_constr i Δ = Some (p, c, P) →
+  (∀ (P'':=P'), P ⊢ P') →
+  match envs_simple_replace i p (Esnoc Enil (c,i) P') Δ with
+  | None => False
+  | Some Δ' => envs_entails Δ' Q
+  end →
+  envs_entails Δ Q.
+Proof.
+  destruct (envs_simple_replace _ _ _ _) as [Δ'|] eqn:Hrep; last done.
+  rewrite envs_entails_eq /=. intros ? HP ?.
+  rewrite envs_simple_replace_singleton_sound_with_constr //; simpl.
+  destruct c; by rewrite ?HP wand_elim_r.
+Qed.
+
+Class AffineEnv (Γ : env PROP) := affine_env : Forall Affine Γ.
+Global Instance affine_env_nil : AffineEnv Enil.
+Proof. constructor. Qed.
+Global Instance affine_env_snoc Γ i P :
+  Affine P → AffineEnv Γ → AffineEnv (Esnoc Γ i P).
+Proof. destruct i as [[] i]; rewrite /AffineEnv;
+       cbn [env_to_list]; by try (constructor).
+Qed.
+
+(* If the BI is affine, no need to walk on the whole environment. *)
+Global Instance affine_env_bi `(BiAffine PROP) Γ : AffineEnv Γ | 0.
+Proof. induction Γ; apply _. Qed.
+
+Instance affine_env_spatial Δ :
+  AffineEnv (env_spatial Δ) → Affine ([∗] env_spatial Δ).
+Proof. intros H. induction H; simpl; apply _. Qed.
+
+Lemma tac_emp_intro Δ : AffineEnv (env_spatial Δ) → envs_entails Δ emp.
+Proof. intros. by rewrite envs_entails_eq (affine (of_envs Δ)). Qed.
+
+Lemma tac_assumption Δ i p P Q :
+  envs_lookup_true i Δ = Some (p,P) →
+  FromAssumption p P Q →
+  (let Δ' := envs_delete true i p Δ in
+   if env_spatial_is_nil Δ' then TCTrue
+   else TCOr (Absorbing Q) (AffineEnv (env_spatial Δ'))) →
+  envs_entails Δ Q.
+Proof.
+  intros ?? H. rewrite envs_entails_eq envs_lookup_sound //.
+  simpl in *. destruct (env_spatial_is_nil _) eqn:?.
+  - by rewrite (env_spatial_is_nil_intuitionistically _) // sep_elim_l.
+  - rewrite from_assumption. destruct H; by rewrite sep_elim_l.
+Qed.
+
+Lemma tac_assumption_coq Δ P Q :
+  (⊢ P) →
+  FromAssumption true P Q →
+  (if env_spatial_is_nil Δ then TCTrue
+   else TCOr (Absorbing Q) (AffineEnv (env_spatial Δ))) →
+  envs_entails Δ Q.
+Proof.
+  rewrite /FromAssumption /bi_emp_valid /= => HP HPQ H.
+  rewrite envs_entails_eq -(left_id emp%I bi_sep (of_envs Δ)).
+  rewrite -bi.intuitionistically_emp HP HPQ.
+  destruct (env_spatial_is_nil _) eqn:?.
+  - by rewrite (env_spatial_is_nil_intuitionistically _) // sep_elim_l.
+  - destruct H; by rewrite sep_elim_l.
+Qed.
+
+Lemma tac_rename Δ i j p c P Q :
+  envs_lookup_with_constr i Δ = Some (p, c, P) →
+  match envs_simple_replace i p (Esnoc Enil (c,j) P) Δ with
+  | None => False
+  | Some Δ' => envs_entails Δ' Q
+  end →
+  envs_entails Δ Q.
+Proof.
+  destruct (envs_simple_replace _ _ _ _) as [Δ'|] eqn:Hrep; last done.
+  rewrite envs_entails_eq=> ??. rewrite envs_simple_replace_singleton_sound_with_constr //.
+  by rewrite wand_elim_r.
+Qed.
+
+Lemma tac_clear Δ i p c P Q :
+  envs_lookup_with_constr i Δ = Some (p,c,P) →
+  (if p then TCTrue else TCOr (TCOr (Affine P) (Absorbing Q))
+                              (if c then (TCOr (Affine P) (Absorbing Q))
+                                    else TCTrue)) →
+  envs_entails (envs_delete true i p Δ) Q →
+  envs_entails Δ Q.
+Proof.
+  rewrite envs_entails_eq=> ? HT HQ. rewrite envs_lookup_sound_with_constr //. rewrite HQ. destruct p, c, HT; cbn in *; by rewrite /= ?sep_elim_r.
+Qed.
+
+(** * False *)
+Lemma tac_ex_falso Δ Q : envs_entails Δ False → envs_entails Δ Q.
+Proof. by rewrite envs_entails_eq -(False_elim Q). Qed.
+
+Lemma tac_false_destruct Δ i p P Q :
+  envs_lookup_true i Δ = Some (p,P) →
+  P = False%I →
+  envs_entails Δ Q.
+Proof.
+  rewrite envs_entails_eq => ??. subst. rewrite envs_lookup_sound //; simpl.
+  by rewrite intuitionistically_if_elim sep_elim_l False_elim.
+Qed.
+
+(** * Pure *)
+Lemma tac_pure_intro Δ Q φ a :
+  FromPure a Q φ →
+  (if a then AffineEnv (env_spatial Δ) else TCTrue) →
+  φ →
+  envs_entails Δ Q.
+Proof.
+  intros ???. rewrite envs_entails_eq -(from_pure a Q). destruct a; simpl.
+  - by rewrite (affine (of_envs Δ)) pure_True // affinely_True_emp affinely_emp.
+  - by apply pure_intro.
+Qed.
+
+Lemma tac_pure Δ i p P φ Q :
+  envs_lookup_true i Δ = Some (p, P) →
+  IntoPure P φ →
+  (if p then TCTrue else TCOr (Affine P) (Absorbing Q)) →
+  (φ → envs_entails (envs_delete true i p Δ) Q) → envs_entails Δ Q.
+Proof.
+  rewrite envs_entails_eq=> ?? HPQ HQ.
+  rewrite envs_lookup_sound //; simpl. destruct p; simpl.
+  - rewrite (into_pure P) -persistently_and_intuitionistically_sep_l persistently_pure.
+    by apply pure_elim_l.
+  - destruct HPQ.
+    + rewrite -(affine_affinely P) (into_pure P) -persistent_and_affinely_sep_l.
+      by apply pure_elim_l.
+    + rewrite (into_pure P) -(persistent_absorbingly_affinely ⌜ _ ⌝%I) absorbingly_sep_lr.
+      rewrite -persistent_and_affinely_sep_l. apply pure_elim_l=> ?. by rewrite HQ.
+Qed.
+
+Lemma tac_pure_revert Δ φ Q : envs_entails Δ (⌜φ⌝ → Q) → (φ → envs_entails Δ Q).
+Proof. rewrite envs_entails_eq. intros HΔ ?. by rewrite HΔ pure_True // left_id. Qed.
+
+
 Lemma tac_forall_intro {A} Δ (Φ : A → PROP) Q :
   FromForall Q Φ →
   (∀ a, envs_entails Δ (Φ a)) →
@@ -22,7 +163,6 @@ Proof.
   rewrite envs_entails_eq /FromForall=> <-.
   apply forall_intro.
 Qed.
-
 
 Lemma tac_impl_intro Δ i P P' Q R :
   FromImpl R P Q →
@@ -36,11 +176,11 @@ Lemma tac_impl_intro Δ i P P' Q R :
 Proof.
   destruct (envs_app _ _ _) eqn:?; last done.
   rewrite /FromImpl envs_entails_eq => <- ???. destruct (env_spatial_is_nil Δ) eqn:?.
-  - rewrite (env_spatial_is_nil_intuitionistically Δ) //; simpl. apply impl_intro_l.
-    rewrite envs_app_singleton_sound //; simpl.
+  - rewrite (env_spatial_is_nil_intuitionistically Δ) //; apply impl_intro_l.
+    rewrite envs_app_singleton_sound //;
     rewrite -(from_affinely P' P) -affinely_and_lr.
     by rewrite persistently_and_intuitionistically_sep_r intuitionistically_elim wand_elim_r.
-  - apply impl_intro_l. rewrite envs_app_singleton_sound //; simpl.
+  - apply impl_intro_l. rewrite envs_app_singleton_sound //;
     by rewrite -(from_affinely P' P) persistent_and_affinely_sep_l_1 wand_elim_r.
 Qed.
 
@@ -59,6 +199,7 @@ Proof.
   rewrite (_ : P = <pers>?false P)%I // (into_persistent false P).
   by rewrite persistently_and_intuitionistically_sep_l wand_elim_r.
 Qed.
+
 Lemma tac_impl_intro_drop Δ P Q R :
   FromImpl R P Q → envs_entails Δ Q → envs_entails Δ R.
 Proof.
@@ -75,7 +216,7 @@ Lemma tac_wand_intro Δ i P Q R :
 Proof.
   destruct (envs_app _ _ _) as [Δ'|] eqn:Hrep; last done.
   rewrite /FromWand envs_entails_eq => <- HQ.
-  rewrite envs_app_sound //; simpl. by rewrite right_id HQ.
+  rewrite envs_app_sound //; simpl; by rewrite right_id HQ.
 Qed.
 
 
@@ -99,22 +240,6 @@ Proof.
       absorbingly_sep_l wand_elim_r HQ.
 Qed.
 
-Lemma tac_assumption Δ i p P Q :
-  envs_lookup_true i Δ = Some (p,P) →
-  FromAssumption p P Q →
-  (let Δ' := envs_delete true i p Δ in
-   if env_spatial_is_nil Δ' then TCTrue
-   else Absorbing Q
-        (* For now not dealing with the case when the whole env can be affine *)
-        (* TCOr (Absorbing Q) (AffineEnv (env_spatial Δ')) *)) →
-  envs_entails Δ Q.
-Proof.
-  intros ?? H. rewrite envs_entails_eq envs_lookup_sound //.
-  simpl in *. destruct (env_spatial_is_nil _) eqn:?.
-  - by rewrite (env_spatial_is_nil_intuitionistically _) // sep_elim_l.
-  - rewrite from_assumption. by rewrite sep_elim_l.
-Qed.
-
 Lemma tac_sep_split Δ bs P Q1 Q2 :
   FromSep P Q1 Q2 →
   match envs_split bs Δ with
@@ -126,6 +251,95 @@ Proof.
   rewrite envs_entails_eq=>? [HQ1 HQ2].
   rewrite envs_split_sound //. by rewrite HQ1 HQ2.
 Qed.
+
+Lemma tac_and_destruct_split Δ i p j1 j2 c c' P P1 P2 Q :
+  envs_lookup_with_constr i Δ = Some (p, c, P) →
+  (IntoAnd p P P1 P2) →
+  match envs_simple_replace i p (Esnoc (Esnoc Enil (negb c' && c, j2) P2)
+                                       (c' && c, j1) P1) Δ with
+  | None => False
+  | Some Δ' => envs_entails Δ' Q
+  end → envs_entails Δ Q.
+Proof.
+  destruct (envs_simple_replace _ _ _ _) as [Δ'|] eqn:Hrep; last done.
+  rewrite envs_entails_eq => H HP HQ.
+  apply pure_elim with (envs_wf Δ).
+  { rewrite of_envs_eq. apply and_elim_l. }
+  move => wf. move: H HP HQ.
+  destruct c.
+  - rewrite envs_lookup_with_constr_envs_lookup_true; [move {wf} => H HP HQ| done].
+    rewrite envs_simple_replace_sound //. destruct p.
+    { rewrite (into_and _ P) HQ. destruct c'; cbn.
+      + by rewrite and_elim_l and_True wand_elim_r.
+      + by rewrite and_elim_r and_True wand_elim_r. }
+    { rewrite (into_and _ P) HQ. destruct c'; cbn.
+      + by rewrite and_elim_l sep_emp wand_elim_r.
+      + by rewrite and_elim_r sep_emp wand_elim_r. }
+  - destruct c'; move => H HP HQ; destruct p;
+    rewrite envs_simple_replace_sound_with_constr //;
+    rewrite HQ ?intuitionistically_True_emp wand_elim_r //=.
+Qed.
+
+Lemma tac_or_l Δ P Q1 Q2 :
+  FromOr P Q1 Q2 → envs_entails Δ Q1 → envs_entails Δ P.
+Proof.
+  rewrite envs_entails_eq=> ? ->. rewrite -(from_or P). by apply or_intro_l'.
+Qed.
+Lemma tac_or_r Δ P Q1 Q2 :
+  FromOr P Q1 Q2 → envs_entails Δ Q2 → envs_entails Δ P.
+Proof.
+  rewrite envs_entails_eq=> ? ->. rewrite -(from_or P). by apply or_intro_r'.
+Qed.
+
+Lemma tac_or_destruct Δ i p j1 j2 c P P1 P2 Q :
+  envs_lookup_with_constr i Δ = Some (p, c, P) → IntoOr P P1 P2 →
+  match envs_simple_replace i p (Esnoc Enil (c, j1) P1) Δ,
+        envs_simple_replace i p (Esnoc Enil (c, j2) P2) Δ with
+  | Some Δ1, Some Δ2 => envs_entails Δ1 Q ∧ envs_entails Δ2 Q
+  | _, _ => False
+  end →
+  envs_entails Δ Q.
+Proof.
+  destruct (envs_simple_replace i p (Esnoc Enil _ P1)) as [Δ1|] eqn:?; last done.
+  destruct (envs_simple_replace i p (Esnoc Enil _ P2)) as [Δ2|] eqn:?; last done.
+  rewrite envs_entails_eq. intros ?? (HP1&HP2).
+  destruct c.
+  - apply pure_elim with (envs_wf Δ).
+    { rewrite of_envs_eq. apply and_elim_l. }
+    move => wf. move: H. rewrite envs_lookup_with_constr_envs_lookup_true //= => H.
+    rewrite envs_lookup_sound //.
+    rewrite (into_or P) intuitionistically_if_or sep_or_r; apply or_elim.
+    + rewrite (envs_simple_replace_singleton_sound' _ Δ1) //.
+      by rewrite wand_elim_r.
+    + rewrite (envs_simple_replace_singleton_sound' _ Δ2) //.
+      by rewrite wand_elim_r.
+  - rewrite (envs_simple_replace_sound_with_constr _ _ _ _ _ _ _ H) //.
+    destruct p; rewrite ?intuitionistically_True_emp wand_elim_r //=.
+Qed.
+
+Lemma tac_exist {A} Δ P (Φ : A → PROP) :
+  FromExist P Φ → (∃ a, envs_entails Δ (Φ a)) → envs_entails Δ P.
+Proof.
+  rewrite envs_entails_eq => ? [a ?].
+  rewrite -(from_exist P). eauto using exist_intro'.
+Qed.
+
+Lemma tac_exist_destruct {A} Δ i p j P (Φ : A → PROP) Q :
+  envs_lookup_true i Δ = Some (p, P) → IntoExist P Φ →
+  (∀ a,
+    match envs_simple_replace i p (Esnoc Enil (true, j) (Φ a)) Δ with
+    | Some Δ' => envs_entails Δ' Q
+    | None => False
+    end) →
+  envs_entails Δ Q.
+Proof.
+  rewrite envs_entails_eq => ?? HΦ. rewrite envs_lookup_sound //.
+  rewrite (into_exist P) intuitionistically_if_exist sep_exist_r.
+  apply exist_elim=> a; specialize (HΦ a) as Hmatch.
+  destruct (envs_simple_replace _ _ _ _) as [Δ'|] eqn:Hrep; last done.
+  rewrite envs_simple_replace_singleton_sound' //; simpl. by rewrite wand_elim_r.
+Qed.
+
 End bi.
 
 
@@ -133,13 +347,6 @@ Import Ltac2.
 Import utils.Misc utils.Iriception utils.Evars.
 
 From Local Require ltac2_tactics.
-
-Ltac2 i_start_split_proof () :=
-  match! goal with
-  | [|- @envs_entails _ _ _] => refine '(@from_named _ _ _) > [ () | () | cbn]
-  | [|- _] => ()
-  end.
-
 
 Ltac2 pm_reduce () :=
   cbv [named_prop.env_spatial named_prop.env_intuitionistic named_prop.env_counter
@@ -154,26 +361,87 @@ Ltac2 pm_reduce () :=
 Ltac2 pm_reflexivity () :=
   pm_reduce (); exact eq_refl.
 
-Ltac2 i_intro_constr (x:constr) :=
-  (failwith (i_start_split_proof) "couldn't start splitting proof in intro_constr");
-  (or
+Ltac2 pm_prettify () :=
+  ltac2_tactics.pm_prettify ().
+
+Ltac2 i_start_split_proof () :=
+  let apply_named () := refine '(from_named _ _ _) > [ pm_reduce ()] in
+  lazy_match! goal with
+  | [|- @environments.envs_entails _ _ _] => apply_named ()
+  | [|- @envs_entails _ _ _] => ()
+  | [|- ?p ] => ltac2_tactics.i_start_proof (); apply_named ()
+  end.
+
+
+Ltac2 i_fresh_fun () :=
+  i_start_split_proof ();
+  lazy_match! goal with
+   | [|- @envs_entails ?pr1 (@Envs ?pr2 ?p ?s ?c) ?q] =>
+    (ltac1:(pr1 pr2 p s c q |-
+           let c1 := (eval vm_compute in (Pos.succ c)) in
+           convert_concl_no_check (@envs_entails pr1 (@Envs pr2 p s c1) q))
+           (Ltac1.of_constr pr1) (Ltac1.of_constr pr2) (Ltac1.of_constr p) (Ltac1.of_constr s) (Ltac1.of_constr c) (Ltac1.of_constr q));
+     constr:(IAnon $c)
+end.
+
+
+Ltac2 i_solve_tc := ltac2_tactics.i_solve_tc.
+
+
+Ltac2 i_intro_pat' (x : Std.intro_pattern) :=
+  or (fun () => failwith (fun () => intros0 false [x]) "couldn't use intro")
+     (fun () =>
+      failwith i_start_split_proof "couldn't start proof in i_intro_pat";
+      lazy_match! goal with
+      | [|- @envs_entails _ _ _] =>
+        refine '(tac_forall_intro _ _ _ _ _) >
+        [ () | ()
+        | orelse i_solve_tc
+          (fun e => lazy_match! goal with
+          | [|- FromForall ?p _ : _] =>
+             Control.zero (Iriception
+                             ((Message.of_string "iIntro: cannot turn ") ++
+                              (Message.of_constr p) ++
+                              (Message.of_string " into a universal quantifier")))
+          end)
+        | pm_prettify (); intros0 false [x] ]
+      end).
+
+Ltac2 Notation "i_intro_pat" p(intropattern) := i_intro_pat' p.
+
+Ltac2 i_intro_constr (x: constr) :=
+  failwith (i_start_split_proof) "Couldn't start splitting proof in intro_constr";
+  or
     (fun () => refine '(@tac_impl_intro _ _ $x _ _ _ _ _ _ _ _) >
-     [() | () | ()
-     | ltac2_tactics.i_solve_tc ()
-     | pm_reduce (); ltac2_tactics.i_solve_tc ()
-     | ltac2_tactics.i_solve_tc ()
-     | pm_reduce ();
-       lazy_match! goal with
-       | [|- False] => Control.zero (Iriception (os "i_intro " ++ oc x ++ os " not fresh"))
-       | [|- _] => ()
-       end])
+            [() | () | ()
+            | i_solve_tc ()
+            | pm_reduce (); ltac2_tactics.i_solve_tc ()
+            | i_solve_tc ()
+            | pm_reduce ();
+              lazy_match! goal with
+              | [|- False] => Control.zero (Iriception (os "i_intro " ++ oc x ++ os " not fresh"))
+              | [|- _] => ()
+               end])
     (fun () => refine '(@tac_wand_intro _ _ $x _ _ _ _ _) >
-     [ () | ()
-     | ltac2_tactics.i_solve_tc ()
-     | pm_reduce ()])).
+            [ () | ()
+            | i_solve_tc ()
+            | pm_reduce ()]).
+
+Ltac2 i_intro_intuitionistic_constr (x : constr) :=
+  failwith (i_start_split_proof)
+           "Couldn't start splitting proof in intro_constr";
+    or (fun () =>
+        refine '(tac_impl_intro_intuitionistic _ $x _ _ _ _ _ _ _) >
+        [ () | () | ()
+        | i_solve_tc () | i_solve_tc ()
+        | pm_reduce ()])
+     (fun () =>
+        refine '(tac_wand_intro_intuitionistic _ $x _ _ _ _ _ _ _ _) >
+        [ () | () | ()
+        | i_solve_tc () | i_solve_tc ()
+        | i_solve_tc () | pm_reduce ()]).
 
 
-Print Ltac2 unify0.
 Ltac2 rec unify_constr_true (e : constr) :=
   lazy_match! e with
   | andb ?b1 ?b2 => (unify0 b1 '(true)); unify_constr_true b2
@@ -185,26 +453,6 @@ Ltac2 rec unify_constr_false (e : constr) :=
   | andb ?b1 ?b2 => (unify0 b1 '(false))
   | ?e => unify0 e '(false)
 end.
-
-Goal True.
-Proof.
-  let v1 := new_evar_with_cast '(bool) in
-  let v2 := new_evar_with_cast '(bool) in
-  assert ($v1 && ($v2 && true) = true).
-  lazy_match! goal with
-  | [|- ?e = true] => unify_constr_true e
-  end.
-  reflexivity.
-  let v1 := new_evar_with_cast '(bool) in
-  let v2 := new_evar_with_cast '(bool) in
-  assert ($v1 && ($v2 && true) = false).
-  lazy_match! goal with
-  | [|- ?e = false] => unify_constr_false e
-  end.
-  reflexivity.
-  constructor.
-  Unshelve. exact false.
-Qed.
 
 Ltac2 i_exact_spatial h :=
   let rec list_from_env e :=
